src/ocaml/extraction/BinNat.mli
@@ -25,7 +25,15 @@ module N :
 
   val ltb : coq_N -> coq_N -> bool
 
+  val even : coq_N -> bool
+
+  val odd : coq_N -> bool
+
   val pos_div_eucl : positive -> coq_N -> coq_N * coq_N
+
+  val div_eucl : coq_N -> coq_N -> coq_N * coq_N
+
+  val div : coq_N -> coq_N -> coq_N
 
   val to_uint : coq_N -> uint
  end
