src/ocaml/extraction/Strings.ml
@@ -1,0 +1,62 @@
+open Ascii
+open BinNat
+open BinNums
+open BinPos
+open Decimal
+open DecimalString
+open PeanoNat
+open String0
+
+(** val newline : char list **)
+
+let newline =
+  (ascii_of_N (Npos (Coq_xO (Coq_xI (Coq_xO Coq_xH)))))::[]
+
+type signed_int =
+| Pos of uint
+| Neg of uint
+
+(** val nat_to_signed_int : int -> signed_int **)
+
+let nat_to_signed_int n =
+  Pos (Nat.to_uint n)
+
+(** val coq_N_to_signed_int : coq_N -> signed_int **)
+
+let coq_N_to_signed_int n =
+  Pos (N.to_uint n)
+
+(** val coq_Z_to_signed_int : coq_Z -> signed_int **)
+
+let coq_Z_to_signed_int = function
+| Z0 -> Pos (Nat.to_uint 0)
+| Zpos m -> Pos (Pos.to_uint m)
+| Zneg m -> Neg (Pos.to_uint m)
+
+(** val string_of_signed_int : signed_int -> char list **)
+
+let string_of_signed_int = function
+| Pos d0 -> NilEmpty.string_of_uint d0
+| Neg d0 -> append ('-'::[]) (NilEmpty.string_of_uint d0)
+
+(** val string_of_nat : int -> char list **)
+
+let string_of_nat n =
+  string_of_signed_int (nat_to_signed_int n)
+
+(** val string_of_N : coq_N -> char list **)
+
+let string_of_N n =
+  string_of_signed_int (coq_N_to_signed_int n)
+
+(** val string_of_Z : coq_Z -> char list **)
+
+let string_of_Z n =
+  string_of_signed_int (coq_Z_to_signed_int n)
+
+module type Printer =
+ sig
+  type t
+
+  val to_string : t -> char list
+ end
