src/DSL.v
@@ -1,11 +1,11 @@
 
 (** Typed CryptoLine. *)
 
-From Coq Require Import List Ascii ZArith OrderedType String Decimal DecimalString.
+From Coq Require Import List Ascii ZArith OrderedType String.
 From mathcomp Require Import ssreflect ssrnat ssrbool eqtype seq ssrfun.
 From nbits Require Import NBits.
 From BitBlasting Require Import Typ TypEnv State BBCommon.
-From ssrlib Require Import Var SsrOrder ZAriths Store FSets FMaps Tactics Seqs Nats.
+From ssrlib Require Import Var SsrOrder ZAriths Store FSets FMaps Tactics Seqs Nats Strings.
 
 Set Implicit Arguments.
 Unset Strict Implicit.
@@ -13,54 +13,6 @@ Import Prenex Implicits.
 
 Declare Scope dsl.
 Delimit Scope dsl with dsl.
-
-
-Section DecimalStringConversions.
-
-  (*
-    Decimal.int is renamed to Decimal.signed_int to avoid name clashes since 8.16.0.
-    Do not use Decimal.int or any function involving Decimal.int to avoid name clashes.
-    See https://github.com/coq/coq/issues/7017.
-   *)
-
-  Local Open Scope string_scope.
-
-  Definition newline := String (Ascii.ascii_of_N 10) EmptyString.
-
-  Variant signed_int := Pos (d : uint) | Neg (d : uint).
-
-  Definition nat_to_signed_int (n : nat) : signed_int := Pos (Nat.to_uint n).
-
-  Definition positive_to_signed_int (n : positive) : signed_int := Pos (Pos.to_uint n).
-
-  Definition N_to_signed_int (n : N) : signed_int := Pos (N.to_uint n).
-
-  Definition Z_to_signed_int (n : Z) : signed_int :=
-    match n with
-    | Z0 => Pos (Nat.to_uint O)
-    | Zpos m => Pos (Pos.to_uint m)
-    | Zneg m => Neg (Pos.to_uint m)
-    end.
-
-  Definition string_of_signed_int (d : signed_int) :=
-    match d with
-    | Pos d => NilEmpty.string_of_uint d
-    | Neg d => String.String "-" (NilEmpty.string_of_uint d)
-    end.
-
-  Definition string_of_nat (n : nat) : string :=
-    string_of_signed_int (nat_to_signed_int n).
-
-  Definition string_of_positive (n : positive) : string :=
-    string_of_signed_int (positive_to_signed_int n).
-
-  Definition string_of_N (n : N) : string :=
-    string_of_signed_int (N_to_signed_int n).
-
-  Definition string_of_Z (n : Z) : string :=
-    string_of_signed_int (Z_to_signed_int n).
-
-End DecimalStringConversions.
 
 
 Section Operators.
@@ -755,12 +707,6 @@ Section DSLRaw.
 
 End DSLRaw.
 
-
-
-Module Type Printer.
-  Parameter t : Type.
-  Parameter to_string : t -> string.
-End Printer.
 
 Module MakeDSL
        (V : SsrOrder)
@@ -8857,11 +8803,5 @@ Module MakeDSL
   End Slicing.
 
 End MakeDSL.
-
-Module VarOrderPrinter <: Printer with Definition t := var.
-  Definition t := VarOrder.t.
-  Definition to_string (v : VarOrder.t) :=
-    ("v" ++ string_of_N v)%string.
-End VarOrderPrinter.
 
 Module DSL := MakeDSL VarOrder VarOrderPrinter VS VM TE Store.
